Working on the informal semantics

Safety.v
@@ -27,6 +27,119 @@ Definition memvis_update mvis ceff :=
   | CEF_Spawn tid => mvis (* TODO *)
   end.
 
+(* ------------------------------------------------------------------------- *)
+
+(*
+Reserved Notation "mt / Gamma '|==' t 'is' mvis"
+  (at level 40, Gamma at next level).
+
+Inductive well_typed_term' (mt : memtyp) : ctx -> tm -> memvis -> Prop :=
+  
+(*
+  | T_Arr : forall Gamma T i,
+    T = get_typ mt i ->
+    i < length mt ->
+    Gamma |-- (TM_Arr (TY_Arr T) i) is (TY_Arr T)
+
+  | T_IArr : forall Gamma T i,
+    T = get_typ mt i ->
+    i < length mt ->
+    Gamma |-- (TM_Arr (TY_IArr T) i) is (TY_IArr T)
+
+  | T_ArrNew : forall Gamma e E,
+    Gamma |-- e is E ->
+    Gamma |-- (TM_ArrNew (TY_Arr E) e) is (TY_Arr E)
+
+  | T_IArrNew : forall Gamma e E,
+    Gamma |-- e is E -> (* immutable *)
+    Gamma |-- (TM_ArrNew (TY_IArr E) e) is (TY_IArr E)
+
+  | T_ArrIdx : forall Gamma arr idx T,
+    Gamma |-- arr is (TY_Arr T) ->
+    Gamma |-- idx is TY_Num ->
+    Gamma |-- (TM_ArrIdx arr idx) is T
+
+  | T_IArrIdx : forall Gamma arr idx T,
+    Gamma |-- arr is (TY_IArr T) ->
+    Gamma |-- idx is TY_Num ->
+    Gamma |-- (TM_ArrIdx arr idx) is T
+
+  | T_Id_Val : forall Gamma id T,
+    lookup Gamma id = Some (TY_IRef T) ->
+    Gamma |-- (TM_Id id) is (TY_IRef T)
+
+  | T_Id_Var : forall Gamma id T,
+    lookup Gamma id = Some (TY_Ref T) ->
+    Gamma |-- (TM_Id id) is (TY_Ref T)
+
+  | T_Asg : forall Gamma t e T,
+    Gamma |-- t is (TY_Ref T) ->
+    Gamma |-- e is T ->
+    Gamma |-- (TM_Asg t e) is TY_Void
+
+  | T_ArrAsg : forall Gamma arr idx e E,
+    Gamma |-- arr is (TY_Arr E) ->
+    Gamma |-- idx is TY_Num ->
+    Gamma |-- e is E ->
+    Gamma |-- (TM_ArrAsg arr idx e) is TY_Void
+
+  | T_Call : forall Gamma f a P R,
+    Gamma |-- f is (TY_Fun P R) ->
+    Gamma |-- a is P ->
+    Gamma |-- (TM_Call f a) is R
+
+  | T_Seq : forall Gamma t t' T,
+    Gamma |-- t  is TY_Void ->
+    Gamma |-- t' is T ->
+    Gamma |-- (TM_Seq t t') is T
+
+  | T_Spawn : forall Gamma block T,
+    safe Gamma |-- block is T ->
+    Gamma |-- (TM_Spawn block) is TY_Void
+
+  | T_LetVal : forall Gamma id e t E T,
+    Gamma |-- e is E ->
+    (update Gamma id E) |-- t is T ->
+    Gamma |-- (TM_LetVal id E e t) is T
+
+  | T_LetVar : forall Gamma id e t E T,
+    Gamma  |-- e is E ->
+    (update Gamma id (TY_Ref E)) |-- t is T ->
+    Gamma  |-- (TM_LetVar id E e t) is T
+
+  | T_LetFun : forall Gamma id F P R f t T,
+    F = TY_Fun P R ->
+    safe Gamma |-- f is F ->
+    (update Gamma id F) |-- t is T ->
+    Gamma |-- (TM_LetFun id F f t) is T
+
+  | T_Loc : forall Gamma i,
+    i < length mt ->
+    Gamma |-- (TM_Loc i) is TY_Ref (get_typ mt i)
+*)
+  | T_Load_Ref : forall Gamma t T,
+    mt / Gamma |-- t is TY_Ref T ->
+    mt / Gamma |== (TM_Load t) is T
+
+  | T_Load_IRef : forall Gamma t T,
+    Gamma |-- t is TY_IRef T ->
+    Gamma |-- (TM_Load t) is T
+*)
+
+Fixpoint f t : list nat :=
+  match t with
+  | TM_Nil => nil
+  | TM_Num _ => nil
+  | TM_Load t' => f t'
+  | TM_Fun p P block R => f block
+  | _ => nil
+  end.
+
+
+(* ------------------------------------------------------------------------- *)
+
+==>
+
 (* trace step (from one concurrent state to another) *)
 Inductive tstep : mem -> threads -> memvis -> trace ->
                   mem -> threads -> memvis -> trace -> Prop :=
@@ -45,13 +158,13 @@ Definition safe_memory_address mt addr :=
   safe_type (get_typ mt addr).
 
 Definition safe_load mt (mvis : memvis) tid addr :=
-  multimap_lookup mvis addr = (tid :: nil) \/
-  safe_memory_address mt addr.
+  safe_memory_address mt addr \/
+  multimap_lookup mvis addr = (tid :: nil).
 
 Definition safe_store (mvis : memvis) tid addr :=
-  multimap_lookup mvis addr = tid :: nil.
+  multimap_lookup mvis addr = (tid :: nil).
 
-Inductive well_formed_trace : mem_typ -> memvis -> trace -> Prop :=
+Inductive well_formed_trace : memtyp -> memvis -> trace -> Prop :=
   | well_formed_trace_nil : forall mt, (* TODO: is this mt correct? *)
     well_formed_trace mt memvis_empty nil
 
@@ -97,7 +210,7 @@ Proof.
     rewrite (get_i_set_j TM_Nil); trivial.
 Qed.
 
-Theorem trace_preservation : forall mt m m' ths ths' mvis mvis' trc trc',
+Theorem safety_preservation : forall mt m m' ths ths' mvis mvis' trc trc',
   well_typed_program mt m ths ->
   well_formed_trace mt mvis trc ->
   m / ths / mvis / trc ~~> m' / ths' / mvis' / trc' ->
@@ -116,7 +229,8 @@ Proof.
       eapply well_formed_trace_alloc; eauto.
     + eexists. eexists. split; eauto using extends_refl.
       eapply well_formed_trace_load; eauto.
-      (* TODO *)
+      unfold safe_load.
+      specialize Hwt as [Hmem Hths].
 Admitted.
 
 
